feat: add BitVec.or

LeanSAT/Reflect/BVExpr/Basic.lean
@@ -7,18 +7,22 @@ import LeanSAT.Reflect.BoolExpr.Basic
 
 inductive BVBinOp where
 | and
+| or
 
 namespace BVBinOp
 
 def toString : BVBinOp → String
   | and => "&&"
+  | or => "||"
 
 instance : ToString BVBinOp := ⟨toString⟩
 
 def eval : BVBinOp → (BitVec w → BitVec w → BitVec w)
   | and => (· &&& ·)
+  | or => (· ||| ·)
 
 @[simp] theorem eval_and : eval .and = ((· &&& ·) : BitVec w → BitVec w → BitVec w) := by rfl
+@[simp] theorem eval_or : eval .or = ((· ||| ·) : BitVec w → BitVec w → BitVec w) := by rfl
 
 end BVBinOp
 
