Test/Bv.lean
@@ -3,12 +3,16 @@ import LeanSAT.Reflect.Tactics.BVDecide
 open BitVec
 
 set_option trace.bv true in
-theorem foo (h1 : 0#1 = 1#1) (h2 : (2 : BitVec 2) = 3) (h3 : x = 4#3)
+theorem unit_1 (h1 : 0#1 = 1#1) (h2 : (2 : BitVec 2) = 3) (h3 : x = 4#3)
     (h4 : x &&& y = y &&& x) : 4#5 = 5#5 := by
   bv_decide
 
 set_option trace.bv true in
-theorem all_features {x y : BitVec 256} (h : x = y) : (~~~x) &&& 1 = (~~~y) &&& 1#256 := by
+theorem unit_2 {x y : BitVec 256} (h : x = y) : (~~~x) &&& 1 = (~~~y) &&& 1#256 := by
+  bv_decide
+
+set_option trace.bv true in
+theorem unit_3 {x y : BitVec 256} : ~~~(x &&& y) = (~~~x ||| ~~~y) := by
   bv_decide
 
 theorem bv_axiomCheck (x : BitVec 1) : x = x := by bv_decide
